more Impl stuff

disk-betree/ImplFlush.i.dfy
@@ -1,9 +1,12 @@
 include "ImplCache.i.dfy"
 include "ImplModelFlush.i.dfy"
+include "ImplFlushRootBucket.i.dfy"
 
 module ImplFlush { 
   import opened Impl
   import opened ImplCache
+  import opened ImplState
+  import opened ImplFlushRootBucket
 
   import opened Options
   import opened MainDiskIOHandler
@@ -17,21 +20,27 @@ module ImplFlush {
   import ImplModel
   import ImplModelCache
   import ImplModelFlush
+  import ImplModelFlushRootBucket
 
-  method flush(k: ImplConstants, s: ImplVariables, io: DiskIOHandler, parentref: BT.G.Reference, slot: int)
+  method flush(k: ImplConstants, s: ImplVariables, parentref: BT.G.Reference, slot: int, childref: BT.G.Reference, child: ImplModel.Node)
   returns (s': ImplVariables)
-  requires IS.Inv(k, s)
-  requires IS.WFVars(s)
+  requires Inv(k, s)
+  requires WFVars(s)
   requires s.Ready?
-  requires parentref in IS.IIndirectionTable(s.ephemeralIndirectionTable)
+
+  requires parentref in IIndirectionTable(s.ephemeralIndirectionTable)
   requires parentref in s.cache
+
   requires s.cache[parentref].children.Some?
   requires 0 <= slot < |s.cache[parentref].buckets|
-  requires io.initialized()
-  requires s.rootBucket == TTT.EmptyTree // FIXME we don't actually need this unless we're flushing the root
-  modifies io
-  ensures IS.WVars(s')
-  ensures ImplModelFlush.flush(IS.Ic(k), old(IS.IVars(s)), old(IS.IIO(io)), parentref, slot) == (IS.IVars(s'), IS.IIO(io))
+  requires s.cache[parentref].children.value[slot] == childref
+
+  requires childref in IIndirectionTable(s.ephemeralIndirectionTable)
+  requires childref in s.cache
+  requires s.cache[childref] == child
+
+  ensures WVars(s')
+  ensures ImplModelFlush.flush(Ic(k), old(IVars(s)), parentref, slot, childref, child) == IVars(s')
   // NOALIAS statically enforced no-aliasing would probably help here
   ensures forall r | r in s.ephemeralIndirectionTable.Repr :: fresh(r) || r in old(s.ephemeralIndirectionTable.Repr)
   modifies s.ephemeralIndirectionTable.Repr
@@ -48,43 +57,34 @@ module ImplFlush {
       }
     }
 
-    var node := s.cache[parentref];
-    var childref := node.children.value[slot];
-    if (childref !in s.cache) {
-      ImplModelCache.lemmaChildInGraph(IS.Ic(k), IS.IVars(s), parentref, childref);
-      // trigger something in Inv about every child pointer points to allocated
-      // indirection record.
-      assert childref in ImplModel.IIndirectionTable(IS.IIndirectionTable(s.ephemeralIndirectionTable)).graph;
-      s' := ImplIO.PageInReq(k, s, io, childref);
-      return;
+    var s1;
+    if parentref == BT.G.Root() {
+      ImplModelFlushRootBucket.flushRootBucketCorrect(Ic(k), IVars(s));
+      s1 := flushRootBucket(k, s);
+    } else {
+      s1 := s;
     }
 
-    var child := s.cache[childref];
-    if (!(
-      && |node.buckets[slot].keys| < 0x4000_0000_0000_0000
-      && |child.buckets| < 0x1_0000_0000_0000_0000
-      && (forall i | 0 <= i < |child.buckets| :: |child.buckets[i].keys| < 0x4000_0000_0000_0000)
-    )) {
-      s' := s;
-      print "giving up; data is 2 big\n";
-      return;
-    }
+    var node := s1.cache[parentref];
+    var childref := node.children.value[slot];
+
+    assume forall i | 0 <= i < |child.buckets| :: |child.buckets[i].keys| + |node.buckets[slot].keys| < 0x8000_0000_0000_0000; // TODO should follow from node weight bound
 
     var newbuckets := KMTable.Flush(node.buckets[slot], child.buckets, child.pivotTable);
     var newchild := child.(buckets := newbuckets);
-    var s1, newchildref := alloc(k, s, newchild);
+    var s2, newchildref := alloc(k, s1, newchild);
     if newchildref.None? {
-      s' := s1;
+      s' := s2;
       print "giving up; could not get parentref\n";
       return;
     }
 
-    var newparent := IS.IM.Node(
+    var newparent := IM.Node(
         node.pivotTable,
         Some(node.children.value[slot := newchildref.value]),
         node.buckets[slot := KMTable.Empty()]
       );
 
-    s' := write(k, s1, parentref, newparent);
+    s' := write(k, s2, parentref, newparent);
   }
 }
